src/TestResult.dfy
@@ -1,23 +1,59 @@
 
+include "../libraries/src/BoundedInts.dfy"
 include "../libraries/src/Wrappers.dfy"
+include "../libraries/src/Collections/Sequences/Seq.dfy"
+include "../libraries/src/Collections/Maps/Maps.dfy"
 
+include "CSV.dfy"
 include "Externs.dfy"
 
 module TestResult {
 
+  import opened BoundedInts
   import opened Wrappers
 
   import Externs
+  import CSV
+  import Maps
+  import Seq
+
+  datatype TestResult = TestResult(displayName: string, outcome: string, durationTicks: int64, resourceCount: nat) {
+    function method ToString(): string {
+      match this
+      case TestResult(displayName, outcome, durationTicks, resourceCount) =>
+        // TODO: extern for formatting duration
+        displayName + "(" + outcome + "): " + Externs.NatToString(resourceCount)
+    }
+  }
+
+  method ParseTestResults(path: string) returns (result: Result<seq<TestResult>, string>) {
+    var lines :- Externs.ReadAllFileLines(path);
+    var table :- CSV.ParseDataWithHeader(lines);
+    result := Seq.MapWithResult(ParseFromCSVRow, table);
+  }
 
   const DISPLAY_NAME := "TestResult.DisplayName";
   const OUTCOME := "TestResult.Outcome";
   const DURATION := "TestResult.Duration";
   const RESOURCE_COUNT := "TestResult.ResourceCount";
 
-  function method ResourceCountOverLimit(testResult: map<string, string>, maximumResourceCount: nat): Result<bool, string> {
-    :- Need(RESOURCE_COUNT in testResult, "Missing ResourceCount entry");
-    var resourceCountStr := testResult[RESOURCE_COUNT];
+  function method GetCSVRowField(row: CSV.Row, fieldName: string): Result<string, string> {
+    :- Need(fieldName in row, "Field missing in row: " + fieldName);
+    Success(row[fieldName])
+  }
+
+  function method ParseFromCSVRow(row: CSV.Row): Result<TestResult, string> {
+    var displayName :- GetCSVRowField(row, DISPLAY_NAME);
+    var outcome :- GetCSVRowField(row, OUTCOME);
+    var durationStr :- GetCSVRowField(row, DURATION);
+    var durationTicks :- Externs.ParseDurationTicks(durationStr);
+    var resourceCountStr :- GetCSVRowField(row, RESOURCE_COUNT);
     var resourceCount :- Externs.ParseNat(resourceCountStr);
-    Success(maximumResourceCount < resourceCount)
+    Success(TestResult(displayName, outcome, durationTicks, resourceCount))
+  }
+
+  predicate method ResourceCountOverLimit(testResult: TestResult, maximumResourceCount: nat) {
+    match testResult
+    case TestResult(_, _, _, resourceCount) => maximumResourceCount < testResult.resourceCount
   }
 }
