src/CSV.dfy
@@ -2,28 +2,33 @@
 include "../libraries/src/Wrappers.dfy"
 include "../libraries/src/Collections/Sequences/Seq.dfy"
 
+include "StandardLibrary.dfy"
 module CSV {
 
   import opened Wrappers
   import opened Seq
+  import opened StandardLibrary
 
-  type CSVRow = map<string, string>
-  type CSVTable = seq<CSVRow>
+  type Row = map<string, string>
+  type Table = seq<Row>
 
-  function method ParseDataWithHeader(lines: seq<string>): Result<CSVTable, string> {
+  function method ParseDataWithHeader(lines: seq<string>): Result<Table, string> {
     :- Need(|lines| > 0, "Must have at least one row");
     var header := ParseRow(lines[0]);
+
     :- Need(|ToSet(header)| == |header|, "Header row must not have duplicates");
     LemmaNoDuplicatesCardinalityOfSet(header);
     var parseRow := line => ParseRowWithHeader(header, line);
+    
     var rows :- Seq.MapWithResult(parseRow, lines[1..]);
     Success(rows)
   }
 
-  function method ParseRowWithHeader(header: seq<string>, line: string): Result<CSVRow, string>
+  function method ParseRowWithHeader(header: seq<string>, line: string): Result<Row, string>
     requires HasNoDuplicates(header)
   {
     var row := ParseRow(line);
+    
     :- Need(|row| == |header|, "Wrong number of columns in row");
     reveal HasNoDuplicates();
     Success(map i | 0 <= i < |header| :: header[i] := row[i])
@@ -31,17 +36,5 @@ module CSV {
 
   function method ParseRow(line: string): seq<string> {
     Split(line, ',')
-  }
-
-  // Could be added to the standard library as well
-  function method {:tailrecursion} Split<T(==)>(s: seq<T>, separator: T): seq<seq<T>> 
-    decreases |s|
-  {
-    var indexOption := IndexOfOption(s, separator);
-    match indexOption
-    case Some(index) =>
-      [s[0..index]] + Split(s[index + 1..|s|], separator)
-    case None =>
-      [s]
   }
 }
