src/Externs.dfy
@@ -13,6 +13,8 @@ module Externs {
   method {:extern} ReadAllFileLines(path: string) returns (lines: Result<seq<string>, string>)
 
   function method {:extern} ParseNat(s: string): Result<nat, string>
-  function method {:extern} ParseDuration(s: string): Result<nat, string>
+  function method {:extern} NatToString(n: nat): string
+  function method {:extern} ParseDurationTicks(s: string): Result<int64, string>
+  function method {:extern} DurationTicksToString(n: int64): string
 }
 
