src/Main.dfy
@@ -1,18 +1,25 @@
 
 include "../libraries/src/Wrappers.dfy"
 include "../libraries/src/BoundedInts.dfy"
+include "../libraries/src/Collections/Sequences/Seq.dfy"
 
 include "CSV.dfy"
 include "Externs.dfy"
+include "StandardLibrary.dfy"
 include "TestResult.dfy"
+
 module Main {
 
   import opened Wrappers
+  import opened Seq
 
   import CSV
   import Externs
-  import TestResult
+  import StandardLibrary
+  import opened TestResult
   
+  datatype Options = Options(maxResourceCount: Option<nat>, filePaths: seq<string>)
+
   method Main() {
     // Working around the lack of arguments or return value on main methods.
     // See https://github.com/dafny-lang/dafny/issues/1116.
@@ -27,23 +34,62 @@ module Main {
   }
 
   method MainAux(args: seq<string>) returns (result: Result<(), string>) {
-    :- Need(|args| == 2, "Not enough arguments.");
-    var path := args[1];
-    result := ProcessFile(path);
-  }
+    var options :- ParseCommandLineOptions(args);
+    
+    // Here I really wish I could use MapWithResult on a method-based Action instead of just a function :(
+    var allResults := [];
+    for pathIndex := 0 to |options.filePaths| {
+      var resultsBatch :- ParseTestResults(options.filePaths[pathIndex]);
+      allResults := allResults + resultsBatch;
+    }
 
-  method ProcessFile(path: string) returns (result: Result<(), string>) {
-    var lines :- Externs.ReadAllFileLines(path);
-    var table :- CSV.ParseDataWithHeader(lines);
-    var passed := true;
-    for i := 0 to |table| {
-      var overlimit :- TestResult.ResourceCountOverLimit(table[i], 2);
-      if overlimit {
-        print "Over the limit: \n", table[i], "\n";
-        passed := false;
+    var resourceCountGetter := (r: TestResult.TestResult) => r.resourceCount;
+    var allResultsSortedByResourceCount := StandardLibrary.MergeSortBy(allResults, resourceCountGetter);
+    
+    print "All results: \n\n";
+    for i := 0 to |allResultsSortedByResourceCount| {
+      print allResultsSortedByResourceCount[i].ToString(), "\n";
+    }
+
+    if options.maxResourceCount.Some? {
+      var allResultsOverLimit := Filter(r => TestResult.ResourceCountOverLimit(r, options.maxResourceCount.value), allResultsSortedByResourceCount);
+      if 0 < |allResultsOverLimit| {
+        print "\n";
+        print "Some results have a resource count over the configured limit of ", options.maxResourceCount.value, ":\n\n";
+        for i := 0 to |allResultsOverLimit| {
+          print allResultsOverLimit[i].ToString(), "\n";
+        }
+        return Failure("\nErrors occurred: see above\n");
       }
     }
-    :- Need(passed, "Some results were over the limit!\n");
+
     return Success(());
+  }
+
+  method ParseCommandLineOptions(args: seq<string>) returns (result: Result<Options, string>) {
+    print args;
+    // For now only one top-level command
+    :- Need(|args| >= 2, "Not enough arguments.");
+    :- Need(args[1] == "summarize-csv-results", "The only supported command is `summarize-csv-results`");
+
+    var maxResourceCount: Option<nat> := None;
+    var filePaths: seq<string> := [];
+    var argIndex := 2;
+    while argIndex < |args| {
+      var arg := args[argIndex];
+      match arg {
+        case "--max-resource-count" => {
+          :- Need(argIndex + 1 < |args|, "--max-resource-count must be followed by the maximum count");
+          argIndex := argIndex + 1;
+          var count :- Externs.ParseNat(args[argIndex]);
+          maxResourceCount := Some(count);
+        }
+        case _ => {
+          filePaths := filePaths + [arg];
+        }
+      }
+      argIndex := argIndex + 1;
+    }
+    return Success(Options(maxResourceCount, filePaths));
   }
 }
