src/StandardLibrary.dfy
@@ -1,0 +1,76 @@
+
+include "../libraries/src/Wrappers.dfy"
+include "../libraries/src/Collections/Sequences/Seq.dfy"
+
+module StandardLibrary {
+
+  import opened Wrappers
+  import opened Seq
+
+  function method {:tailrecursion} Split<T(==)>(s: seq<T>, separator: T): seq<seq<T>> 
+    decreases |s|
+  {
+    var indexOption := IndexOfOption(s, separator);
+    match indexOption
+    case Some(index) =>
+      [s[0..index]] + Split(s[index + 1..|s|], separator)
+    case None =>
+      [s]
+  }
+
+  // TODO: These are not very generic since there's no type characteristic for "comparable".
+  // This version is all I need here, but this could be more general if a comparison function
+  // was provided instead.
+
+  predicate SortedBy<T>(s: seq<T>, f: T -> int) {
+    forall i, j | 0 <= i < j < |s| :: f(s[i]) <= f(s[j])
+  }
+
+  lemma NewFirstElementStillSortedBy<T>(x: T, s: seq<T>, f: T -> int) 
+    requires SortedBy(s, f)
+    requires |s| == 0 || f(x) <= f(s[0])
+    ensures SortedBy([x] + s, f)
+  {}
+
+  function method MergeSortBy<T>(s: seq<T>, f: T -> int): (result: seq<T>)
+    ensures SortedBy(result, f)
+    ensures multiset(s) == multiset(result)
+  {
+    if |s| <= 1 then
+      s
+    else
+      var splitIndex := |s| / 2;
+      var left := s[..splitIndex];
+      var right := s[splitIndex..];
+      assert s == left + right;
+
+      var leftSorted := MergeSortBy(left, f);
+      var rightSorted := MergeSortBy(right, f);
+      
+      MergeSortedBy(leftSorted, rightSorted, f)
+  }
+
+  // TODO: How to add {:tailrecursion} while keeping the assertions necessary to prove the post-conditions?
+  function method MergeSortedBy<T>(left: seq<T>, right: seq<T>, f: T -> int): (result: seq<T>)
+    requires SortedBy(left, f)
+    requires SortedBy(right, f)
+    ensures SortedBy(result, f)
+    ensures multiset(left + right) == multiset(result)
+  {
+    if |left| == 0 then
+      right
+    else if |right| == 0 then
+      left
+    else if f(right[0]) < f(left[0]) then
+      var rest := MergeSortedBy(left, right[1..], f);
+      var result := [right[0]] + rest;
+      NewFirstElementStillSortedBy(right[0], rest, f);
+      assert right == [right[0]] + right[1..];
+      result
+    else
+      var rest := MergeSortedBy(left[1..], right, f);
+      NewFirstElementStillSortedBy(left[0], rest, f);
+      assert left == [left[0]] + left[1..];
+      [left[0]] + rest
+  }
+}
